Incorporated, from J, improvements to comments and :doc pertaining to evaluation (badges, warrants, attachments, program vs. logic mode, etc.).
In addition to adding and modifying lots of source comments and
documentation pertaining to evaluation, J contributed a new :doc topic
-- quoting :doc note-8-5:

  A new documentation topic, guarantees-of-the-top-level-loop, explains
  the logical meaning of evaluation in the ACL2 read-eval-print loop,
  including discussion of attachments (see [defattach]), [badge]s,
  [warrant]s.

books/system/doc/acl2-doc.lisp
@@ -5198,7 +5198,7 @@ and @(tsee include-book)"
 
   <ul>
 
-  <li>@('apply$') -- the ACL2 function that takes two arguments, one
+  <li>@('apply$') &mdash; the ACL2 function that takes two arguments, one
       representing a function and the other listing actuals to be fed to that
       function.  Under certain conditions, @('apply$') applies the function to
       the arguments and returns the result.  @('Apply$') is mutually recursive
@@ -5207,10 +5207,9 @@ and @(tsee include-book)"
       its arity is 2, its ``out arity'' is 1 (i.e., it returns 1 result), its
       first argument has ``ilk'' @(':FN') and is thus treated as a
       ``function;'' its second argument has ilk @('NIL') and is thus treated as
-      an ordinary object.  Initially, @('apply$') is the only symbol in ACL2
-      with an ilk of @(':FN').</li>
+      an ordinary object.</li>
 
-  <li>@(tsee badge) -- an object associated with some function symbols
+  <li>@(tsee badge) &mdash; an object associated with some function symbols
       indicating that @('apply$') can ``handle'' them and under what
       conditions.  The badge of a function symbol specifies its arity, its
       ``out arity,'' (i.e., the number of results the function returns), and
@@ -5223,31 +5222,33 @@ and @(tsee include-book)"
       badges cannot be @('apply$')d.  Badges are generated, when possible, by
       @(tsee defwarrant).  (Badges can be generated for @(':')@('program') mode
       functions by @(tsee defbadge), allowing @('apply$') to handle such
-      functions in top level evaluation not not in proofs.)  Not every function
+      functions in top level evaluation not in proofs.)  Not every function
       symbol can have a badge.</li>
 
-  <li>compiled @('LAMBDA') cache (or simply <i>cache</i> in this context) -- a
+  <li>compiled @('LAMBDA') cache (or simply <i>cache</i> in this context) &mdash; a
       cache in the raw Lisp under ACL2 that supports the application of
       @('apply$') on well-formed, guard verified @('LAMBDA') objects.  Later in
       this Glossary we define ``lambda expression,'' ``@('LAMBDA') object,''
-      and ``lambda$ expression'' -- three similar looking phrases with very
+      and ``lambda$ expression'' &mdash; three similar looking phrases with very
       different meanings.  See @(tsee print-cl-cache) for some details of the
       cache.</li>
 
-  <li>evaluation theory -- the logical theory in which expressions submitted at
-      the top level of the ACL2 read-eval-print loop are evaluated.  The
-      evaluation theory is a consistent extension of the proof theory, the
-      latter being the logical theory in which the ACL2 theorem prover
-      operates.  The evaluation theory is not new to @('apply$'); it was
-      introduced when @(tsee defattach) was added.  But the evaluation theory
-      changed with the introduction of @('apply$').  All @(tsee warrant)s
-      introduced by @('defwarrant') are assumed true in the evaluation theory
-      but not in the proof theory.  This means ACL2 can execute calls of
-      @('apply$') that arise in the evaluation of top-level input, but ACL2
-      cannot evaluate all calls of @('apply$') that arise in proofs unless the
-      appropriate warrants are available as hypotheses.</li>
+  <li>evaluation theory &mdash; the logical theory in which expressions
+      submitted at the top level of the ACL2 read-eval-print loop are
+      evaluated.  The evaluation theory is a consistent extension of the proof
+      theory, the latter being the logical theory in which the ACL2 theorem
+      prover operates.  The evaluation theory was introduced in ACL2 when
+      @(tsee defattach) was added, but it was changed with the introduction of
+      @('apply$').  All @(tsee warrant)s introduced by @('defwarrant') are
+      assumed true in the evaluation theory but not in the proof theory.  This
+      means ACL2 can execute calls of @('apply$') that arise in the evaluation
+      of top-level input, but ACL2 cannot evaluate all calls of @('apply$')
+      that arise in proofs unless the appropriate warrants are available as
+      hypotheses.  See @(see guarantees-of-the-top-level-loop) for some details
+      of the evaluation theory and how it differs from the proof theory
+      supported by the ACL2 theorem prover.</li>
 
-  <li>lambda expression -- an integral part of ACL2's formal term syntax,
+  <li>lambda expression &mdash; an integral part of ACL2's formal term syntax,
       lambda expressions are the way @('let') expressions and other
       variable-binding idioms are translated into formal terms.  Lambda
       expressions have nothing to do with @('apply$')!  See @(see lambda) for a
@@ -5255,22 +5256,22 @@ and @(tsee include-book)"
       expressions, @('LAMBDA') objects, and @('lambda$') expressions.  Read
       carefully anytime you see the word ``lambda!''</li>
 
-  <li>@('LAMBDA') object -- an ACL2 list constant, typically of the form
+  <li>@('LAMBDA') object &mdash; an ACL2 list constant, typically of the form
       @('(LAMBDA vars body)') or @('(LAMBDA vars dcl body)') that may be used
       as a ``function'' by @('apply$').  @('Apply$') treats any @(tsee consp)
       object in its first argument position as though it were a @('LAMBDA')
       object.  But it only gives sensible meanings to @(see tame) @('LAMBDA')
       objects.  And only well-formed @('LAMBDA') objects are executed
       efficiently.  But well-formed @('LAMBDA') objects are hard to type by
-      hand -- there are many constraints to keep in mind to guarantee
+      hand &mdash; there are many constraints to keep in mind to guarantee
       well-formedness.  See @(tsee well-formed-lambda-objectp) if you really
       want to see all the rules.  But that is generally unnecessary.  We
       <i>strongly</i> recommend not entering @('LAMBDA') objects as quoted
-      constants, e.g., @(''(LAMBDA (X) (+ 1 X))') -- which is actually
+      constants, e.g., @(''(LAMBDA (X) (+ 1 X))') &mdash; which is actually
       ill-formed!  Instead, use @(tsee lambda$), as in @('(lambda$ (x) (+ 1
       x))').  See also @(see lambda) for some clarifications.</li>
 
-  <li>@(tsee lambda$) expression -- an ACL2 macro that allows you to enter
+  <li>@(tsee lambda$) expression &mdash; an ACL2 macro that allows you to enter
       quoted well-formed @('LAMBDA') objects into your terms by typing
       untranslated expressions that resemble lambda expressions.  The
       @('lambda$') expression @('(lambda$ (x) (+ 1 x))') essentially translates
@@ -5281,8 +5282,8 @@ and @(tsee include-book)"
       translated @('lambda$'). See also @(see lambda) for some
       clarifications.</li>
 
-  <li>@(tsee scion) -- a function that is ancestrally dependent on @('apply$').
-      In the early days of @('apply$') we called scions ``mapping function''
+  <li>@(tsee scion) &mdash; a function that is ancestrally dependent on @('apply$').
+      In the early days of @('apply$') we called scions ``mapping functions''
       but in the Lisp community that implies iteration over a list and scions
       are more general.  Of course, a function that iterates over a list
       @('apply$')ing a ``function'' to each element and collecting the results
@@ -5291,7 +5292,7 @@ and @(tsee include-book)"
       Any function ancestrally dependent on @('apply$') is a scion whether or
       not it takes a ``function'' as an argument or maps over a domain.</li>
 
-  <li>@(see tame) -- the class of functions that @('apply$') knows about; we
+  <li>@(see tame) &mdash; the class of functions that @('apply$') knows about; we
       actually talk about ``tame functions,'' ``tame @('LAMBDA') objects,'' and
       ``tame expressions.''  The last are expressions that are evaluable by an
       interpreter named @(tsee ev$) that is mutually-recursive with @('apply$').
@@ -5299,7 +5300,7 @@ and @(tsee include-book)"
       and if @('apply$') were able to ``handle'' certain functions the logic
       would be inconsistent.</li>
 
-  <li>@(tsee warrant) -- a 0-ary predicate associated with some user-defined
+  <li>@(tsee warrant) &mdash; a 0-ary predicate associated with some user-defined
       function symbols that must be a hypothesis of any theorem whose proof
       involves ``expanding'' @('apply$') on such symbols; the warrant gives
       @('apply$') ``permission'' to expand if the arguments to which the
@@ -5460,11 +5461,12 @@ and @(tsee include-book)"
   unbadged functions, etc.  They are, after all, just arbitrary quoted objects
   and any value in ACL2 can be quoted.  But an ill-formed object can
   <i>become</i> well-formed if the world is appropriately extended, e.g., the
-  appropriate @('defun')s or @('defwarrant')s are made.  Perhaps worse, they
-  can be well-formed and then <i>become</i> ill-formed by an undo.  So at
-  runtime @('apply$') has to check that the function symbol or @('LAMBDA')
-  object is appropriate.  There is a sophisticated cache behind the execution
-  machinery for @('LAMBDA') objects in the evaluation theory.</p>
+  appropriate @('defun')s, @('defbadge')s, and @('defwarrant')s are made.
+  Perhaps worse, they can be well-formed and then <i>become</i> ill-formed by
+  an undo.  So at runtime @('apply$') has to check that the function symbol or
+  @('LAMBDA') object is appropriate.  There is a sophisticated cache behind the
+  execution machinery for @('LAMBDA') objects in the evaluation theory.  See
+  @(tsee print-cl-cache).</p>
 
   <p>Here are some theorems that can be proved about these concepts.  The last
   of the theorems shown below requires two lemmas, named
@@ -5553,14 +5555,16 @@ and @(tsee include-book)"
   <p>The @(see ilk)s of @('apply$') are @(':FN') and @('NIL') respectively,
   telling us that @('apply$') treats its first argument as a ``function'' and
   its second as an ordinary object (never as a function).  Initially
-  @('apply$') is the only symbol in ACL2 with an ilk of @(':FN').  However as
-  @(tsee defwarrant) is used successfully on @(see scion)s -- functions that
-  somehow call @('apply$') -- other symbols can have ilk @(':FN') too.</p>
+  @('apply$') and several functions used in the translation of @('loop$')
+  statements are the only symbols in ACL2 with an ilk of @(':FN').  However as
+  @(tsee defwarrant) is used successfully on @(see scion)s &mdash; functions that
+  somehow call @('apply$') &mdash; user-defined symbols can have ilk @(':FN')
+  too.</p>
 
   <p>@('Apply$') has a guard, namely @('(apply$-guard fn args)').  This is an
   exceptionally weak guard, requiring only that @('args') be a true-list and,
-  if @('fn') is a cons -- which is automatically treated as a @('LAMBDA')
-  object -- the length of @('args') be the length of the second element of
+  if @('fn') is a cons &mdash; which is automatically treated as a @('LAMBDA')
+  object &mdash; the length of @('args') be the length of the second element of
   @('fn').  We discuss <b>guards and guard verification</b> in a subsequent
   section.</p>
 
@@ -5584,9 +5588,9 @@ and @(tsee include-book)"
   in some theorem, use @('tamep-functionp').  But when you write concrete
   @('LAMBDA') constants, try to keep them well-formed.  We encourage this by
   providing @(tsee lambda$) and by enforcing full blown well-formedness checks
-  -- not just tameness checks -- in translate on every quoted @('LAMBDA')
+  &mdash; not just tameness checks &mdash; in translate on every quoted @('LAMBDA')
   object entered in a @(':FN') slot.  And we give you ways to circumvent these
-  checks -- see @(see gratuitous-lambda-object-restrictions) -- if you really
+  checks &mdash; see @(see gratuitous-lambda-object-restrictions) &mdash; if you really
   mean to supply ill-formed @('LAMBDA') objects to @(':FN') slots.</p>
 
   <p>Badges are assigned by @(tsee defwarrant), and also by @(tsee defbadge).
@@ -5619,7 +5623,8 @@ and @(tsee include-book)"
   want to @('apply$') a @(':program') mode function you should define it with
   @('defun') and then call @('defbadge') on its name.</p>
 
-  <p>We summarize specification of @('apply$') with an example.  Consider</p>
+  <p>We summarize the specification of @('apply$') with an example.
+  Consider</p>
 
   @({  (apply$ 'foldr
           '((1 2 3)     ; actual 1
@@ -5694,7 +5699,7 @@ and @(tsee include-book)"
   function for the function it analyzed.  Warrants are crucial to stating and
   proving theorems about function symbols being applied with @('apply$').  We
   illustrated warrants in the ``Examples'' section above and discuss them
-  further in the secion on ``Theorems Involving @('Apply$')'' below.  See also
+  further in the section on ``Theorems Involving @('Apply$')'' below.  See also
   @(tsee warrant).</p>
 
   <p>@('Apply$') is a defined function in the ACL2 source code.  We exhibit its
@@ -5755,7 +5760,7 @@ and @(tsee include-book)"
   <p>In one sense, @('apply$') is just an ordinary ACL2 function that takes two
   arguments and returns one result.  Like all ACL2 functions, @('apply$') is
   untyped.  You can supply any two objects as arguments and the axioms tell you
-  what the result is -- though sometimes the result is delivered by an
+  what the result is &mdash; though sometimes the result is delivered by an
   undefined function.</p>
 
   <p>But in a deeper sense, if you want @('apply$') to ``behave,'' and in
@@ -5775,7 +5780,7 @@ and @(tsee include-book)"
   <p>So the question becomes ``What rules must a @('defun') obey in order to be
   processed successfully by @('defwarrant')?''  The full answer is given in the
   documentation for @(tsee defwarrant).  But here are some guidelines to
-  follow:
+  follow:</p>
 
   <ul>
   <li>use @(':logic') mode,</li>
@@ -5791,7 +5796,7 @@ and @(tsee include-book)"
   <li>ensure that every parameter passed into a @(':FN') slot is passed into
       the same argument position in any recursive calls of the function being
       defined.</li>
-  </ul></p>
+  </ul>
 
   <p>You can certainly violate some of these rules and still get an admissible
   definition.  For example @('(defun rus (x) (not (apply$ x (list x))))') is
@@ -5799,6 +5804,16 @@ and @(tsee include-book)"
   evaluates to @('T').  You can even prove @('(equal (rus 'consp) t)').  But
   @('(defwarrant rus)') fails because @('rus') violates the rules.  So you will
   not be able to @('apply$') @(''rus').</p>
+
+  <p><b>Note for Experts</b>: One may wonder why it is possible to warrant a
+  function, @('fn'), that calls badged but unwarranted functions.  Naively one
+  might expect the semantics of @('(apply$ 'fn args') would involve the
+  @('ev$') of the body of @('fn') and therefore require the successful
+  application (via @('apply$')) of subfunctions in the body.  But that
+  expectation is incorrect.  The semantics of @('(apply$ 'fn args)') as
+  formalized by the warrant for @('fn') says that (under restrictions on the
+  tameness of the arguments) @('(apply$ 'fn args)') is @('(fn (car args) (cadr
+  args) ...)').</p>
 
   <h3>Theorems Involving @('Apply$')</h3>
 
@@ -5895,10 +5910,12 @@ and @(tsee include-book)"
 
   <p><b>Lesson 3:</b> If a proof involving @('apply$') or a scion fails in a
   forcing round with a checkpoint whose conclusion is the warrant for some
-  function, you should remember Lesson 1 and include that function symbol in
-  the warrant for your conjecture!  That is, if you forget to supply a warrant
-  but your conjecture is otherwise provable, ACL2's checkpoints will remind
-  you.</p>
+  function, you should remember Lesson 1 and include the warrant for that
+  function symbol in the hypotheses of your conjecture!  That is, if you forget
+  to supply a warrant but your conjecture is otherwise provable, ACL2's
+  checkpoints will often remind you.  (It is possible, in the absence of an
+  explict warrant hypothesis, for a proof to fail before the prover detects that
+  only the warrant is missing.)</p>
 
   <p><b>Lesson 4:</b> If a proof involving @('apply$') or a scion fails here
   are some things to think about.  The basic question is whether something is
@@ -5948,8 +5965,8 @@ and @(tsee include-book)"
   <p>The definition of @('my-len') fails!  The reason is that without the
   warrant for @('my-cdr') we cannot prove that the measure decreases in the
   recursion above.  Unfortunately, there is no way to provide a warrant in a
-  definition.  At the moment we advise users to avoid the use of @('apply$') --
-  and functions that use @('apply$') -- in ``termination-critical'' roles.  By
+  definition.  At the moment we advise users to avoid the use of @('apply$') &mdash;
+  and functions that use @('apply$') &mdash; in ``termination-critical'' roles.  By
   that we mean do not use @('apply$') if its properties are important to proofs
   of your measure conjectures.  This is easy advice to implement in the case of
   @('my-len'), i.e., replace the recursive call above by @('(my-len (my-cdr
@@ -6037,10 +6054,10 @@ and @(tsee include-book)"
   scion, e.g., @('(my-scion 'SQU x)').  To what arguments will @('my-scion')
   @('apply$') @('SQU')?  And how can the definition of @('my-scion') even
   specify what functional objects are acceptable in its first argument?  This
-  is a limitation suffered by ACL2 that a suitably expressive type system would
-  not.  Our way of coping with it is to ignore the guard here and make sure
-  that when @('apply$') applies the function symbol executes it checks the
-  guard of the symbol.</p>
+  is a limitation suffered by ACL2 that a logic with a suitably expressive type
+  system would not suffer.  Our way of coping with it is to ignore the guard
+  here and make sure that when @('apply$') applies the function symbol executes
+  it checks the guard of the symbol.</p>
 
   <p>Guard verification does not ignore guards of a quoted lambda object being
   @('apply$')ed.  Thus, for example, while @('strange') can be guard
@@ -6179,28 +6196,35 @@ and @(tsee include-book)"
   <h3>Top-Level Evaluation of Apply$</h3>
 
   <p>As noted, ACL2's evaluation theory implicitly assumes all warrants
-  produced by @(tsee defwarrant).  Since top-level evaluation in ACL2 is
-  conducted in the evaluation theory, ground calls of @('apply$') -- whether
-  literally in top-level input to the ACL2 read-eval-print loop or hidden
-  inside scions called from the top-level -- can be evaluated on quoted
-  warranted function symbols and @(tsee lambda$) expressions -- provided the
-  @(see tame)ness restrictions are met.  This is in contrast to opportunities
-  for evaluation of ground @('apply$') expressions arising in proofs, where
-  warrants must be explicit.</p>
+  produced by @(tsee defwarrant).  See @(see
+  guarantees-of-the-top-level-loop). Since top-level evaluation in ACL2 is
+  conducted in the evaluation theory, ground calls of @('apply$') &mdash;
+  whether literally in top-level input to the ACL2 read-eval-print loop or
+  hidden inside scions called from the top-level &mdash; can be evaluated on
+  quoted warranted function symbols and @(tsee lambda$) expressions &mdash;
+  provided the @(see tame)ness restrictions are met.  This is in contrast to
+  opportunities for evaluation of ground @('apply$') expressions arising in
+  proofs, where warrant hypotheses must be explicit.</p>
 
   <p>In this section we focus on calls of @('apply$') arising in the evaluation
-  theory.  We start with a discussion of the use of @('apply$') with badged
+  theory.  We start with a discussion of the use of @('apply$') with warranted
   @(':logic') mode functions.  We then describe how @('apply$') handles badged
-  @(':program') mode functions.</p>
+  @(':program') mode functions.  Note that a mere badge is <i>not</i>
+  sufficient for evaluation when using @('apply$') on a @(':logic') mode
+  function that is not warranted; see @(tsee defbadge) and @(see
+  guarantees-of-the-top-level-loop) for discussion of this case.  In short:
+  evaluation involving @(':logic') mode functions is expected to respect the
+  evaluation theory, and while @('defwarrant') extends the evaluation theory
+  appropriately, @('defbadge') does not.</p>
 
   <p>Evaluation of @('apply$') terms in the evaluation theory respects guards
   on quoted function symbols and @(tsee lambda$) expressions (which is to say,
   on the quoted well-formed @('LAMBDA') objects that @(tsee lambda$) produces).
   So consider a call of @('apply$') on @('fn') and @('args') in the evaluation
-  theory, where @('fn') is a badged function symbol or a well-formed (and thus
-  tame) @('LAMBDA') object.  Here's what happens.  Except where noted, the
-  description below applies both to badged @(':logic') and badged @(':program')
-  mode functions.</p>
+  theory, where @('fn') is a warranted function symbol or a well-formed (and
+  thus tame) @('LAMBDA') object.  Here's what happens.  Except where noted, the
+  description below applies both to warranted @(':logic') and badged
+  @(':program') mode functions.</p>
 
   <p>@('Apply$') determines whether @('fn')'s tameness restrictions are met by
   @('args').  Tameness is a syntactic property and so can be checked.  If the
@@ -6210,10 +6234,10 @@ and @(tsee include-book)"
   @('fn') has been guard verified.  In the case of function symbols this is a
   simple lookup on the property list of @('fn').  (Of course, this check fails
   for @(':program') mode functions.)  In the case of @('LAMBDA') objects it is
-  a cache query and if the query reveals that we have not yet tried to verify
-  the guards of this @('LAMBDA') object, @('apply$') uses tau reasoning
-  alone (see @(see introduction-to-the-tau-system)) to verify the guard
-  conjectures.</p>
+  a cache query (see @(tsee print-cl-cache)) and if the query reveals that we
+  have not yet tried to verify the guards of this @('LAMBDA') object,
+  @('apply$') uses tau reasoning alone (see @(see
+  introduction-to-the-tau-system)) to try to verify the guard conjectures.</p>
 
   <p><b>Note:</b>An important distinction between the runtime handling of
   function symbols versus @('LAMBDA') objects by @('apply$') is that function
@@ -6242,7 +6266,9 @@ and @(tsee include-book)"
   <p>We discuss the cache that supports @('LAMBDA') application in @(tsee
   print-cl-cache).  See also the discussion of guard verification in @(tsee
   lambda$).  It should be noted that a @('LAMBDA') object can also be guard
-  verified using the @(tsee verify-guards) event.</p>
+  verified using the @(tsee verify-guards) event.  This brings the full power
+  of the prover to bear on the guard verification of the @('LAMBDA') object,
+  instead of relying just on the tau system.</p>
 
   <p>Users are accustomed to executing @(':program') mode functions at the
   top-level of the ACL2 read-eval-print loop.  Indeed, the prover itself and
@@ -6251,22 +6277,28 @@ and @(tsee include-book)"
   theory, i.e., as an axiomatic theory.  And yet no part of that axiomatization
   explains how @(':program') mode functions are run!  It simply isn't
   important.  The implementation supports it and no questions are asked.  We,
-  the implementors of ACL2, view top-level evaluation of both @(':logic') mode
-  and @(':program') mode functions as a convenience not affecting the
-  consistency of the proof theory.  No inconsistency results from starting a
-  non-terminating computation because you can never inspect the result, whereas
-  if you added the corresponding definition as an axiom you might be able to
-  prove something contradictory.  So we regard the seamless execution of
-  @(':program') mode functions as a convenience to the user who might use them
-  to inspect the ACL2 logical world, gather data, experiment with constrained
-  formal models by attaching executable code to unspecified functions,
-  prototype something to be formalized, etc.  In that spirit, we have arranged
-  for @('apply$') to handle @(':program') mode functions <i>provided they have
-  badges</i>.  Badges are critical because it means that execution of the
-  functions won't ``go outside the sandbox.''  However, @('apply$') runs
-  @(':program') mode functions in @(tsee safe-mode) to ensure the functional
-  substitutivity of @('apply$'): identical calls must always yield identical
-  results.</p>
+  the implementors of ACL2, view top-level evaluation of @(':program') mode
+  functions as a convenience not affecting the consistency of the proof theory.
+  No inconsistency results from starting a non-terminating computation because
+  you can never inspect the result, whereas if you added the corresponding
+  definition as an axiom you might be able to prove something contradictory.
+  So we regard the seamless execution of @(':program') mode functions as a
+  convenience to the user who might use them to inspect the ACL2 logical world,
+  gather data, experiment with constrained formal models by attaching
+  executable code to unspecified functions, prototype something to be
+  formalized, etc.  In that spirit, we have arranged for @('apply$') to handle
+  @(':program') mode functions <i>provided they have badges</i>.  Badges are
+  critical because it means that execution of the functions won't ``go outside
+  the sandbox.''  However, @('apply$') runs @(':program') mode functions in
+  @(tsee safe-mode) to ensure the functional substitutivity of @('apply$'):
+  identical calls must always yield identical results.</p>
+
+  <p>It may seem counterintuitive that a top-level @('apply$') of a @(':logic')
+  mode function cannot be executed unless @('defwarrant') has succeeded but a
+  top-level @('apply$') of a @(':program') mode function can be executed.  As
+  noted earlier, the reason is simple: execution of @(':logic') mode functions
+  is justified by the axioms of the evaluation theory while no such assurances
+  are offered for @(':program') mode functions.</p>
 
   <h3>Logical Definitions</h3>
 
@@ -20928,26 +20960,58 @@ subtree of X with T, without duplication.</p>
 
   <h3>Badges versus Warrants</h3>
 
-  <p>It is easy to confuse badges, which are issued by @('defbadge'), with
-  warrants, which are issued by @(tsee defwarrant).  The thing to keep in mind
-  is that badges extend the syntax and evaluation capabilities of ACL2, while
-  warrants extend the proof theory.  Some user-defined function symbols may be
-  given badges even if they are in @(':')@(tsee program) mode (see @(see
-  mixed-mode-functions)).  If @('fn') has a badge, you are allowed to write
-  @('(apply$ 'fn (list a1 ... an))') and expect it evaluate ``correctly'' at
-  the top level of the ACL2 read-eval-print loop, just as you expect @('(fn a1
-  ... an)') to evaluate.  But you cannot <i>prove</i> anything interesting
-  about @('(apply$ 'fn (list a1 ... an))') without the warrant for @('fn').  A
-  badged but unwarranted function symbol might as well be undefined as far as
-  the prover is concerned.  Warrants connect the quoted symbol to the axiomatic
-  behavior of @('apply$'), in particular, they constrain @('(apply$ 'fn (list
-  a1 ... an))') to be @('(fn a1 ... an)') under certain conditions.  Obviously,
-  the very first requirement on @('fn') to have a warrant is that @('fn') must
-  be in @(':')@(tsee logic) mode.  But there are other requirements because
-  @('defwarrant') must make sure the extended proof theory is consistent.</p>
+  <p>It is easy to confuse @(see badge)s, which are issued by @('defbadge'),
+  with @(see warrant)s, which are issued by @(tsee defwarrant).  Badges and
+  warrants are necessary to ACL2's support of @(tsee apply$) because ACL2 is
+  actually first-order, functions cannot be passed around as objects, ordinary
+  symbols play the role of ``function objects,'' and somehow the logic must
+  allow the association of a symbol with the function it names.  Furthermore,
+  to insure the consistency of the logic @('apply$') is not allowed to handle
+  certain functions such as the @('russell') function illustrated in @(tsee
+  introduction-to-apply$).  But to determine whether a newly defined function
+  is allowed to be known to @('apply$'), the ACL2 system must be able to
+  determine, in some sense, all the functions reachable from it.  And finally,
+  to be able to prove theorems about the application of such function names,
+  the link between the symbols and the functions and the analyzed properties of
+  the functions must available to the prover in the form of axioms.
+  Particularly vexing is the so-called ``@('local') problem'' which raises the
+  possibility of proving a theorem about the application of a name in the
+  context of a local definition of the corresponding function and then
+  exporting that theorem to a context where the name is defined
+  differently (see <b>Lesson 12</b> of @(see introduction-to-apply$)).</p>
+
+  <p>Roughly speaking, badges are about syntax and warrants are about
+  semantics.  The badge for a symbol is a data structure in the ACL2 system
+  that records information like whether the symbol names a known ACL2 function,
+  how many arguments that function takes, how many results it returns, which
+  arguments are treated like function objects to be @(tsee apply$)'d, which are
+  treated like expressions to be @(tsee ev$)'d, and which are treated like
+  ordinary ACL2 objects to be @('car')'d, @('cdr')'d, consed, etc.  The
+  warrant for a function is in fact another function (actually a 0-ary
+  predicate) defined in the logic.  That predicate asserts some facts about the
+  symbol.  In particular, it specifies the badge of the symbol and it
+  constrains the behavior of @('apply$') on the symbol.</p>
+
+  <p>@('Defbadge') analyzes the definition of a function and constructs the
+  badge if possible.  @('Defbadge') does not affect the logic &mdash; no
+  definitions or axioms are added.  @('Defbadge') can analyze both
+  @(':program') mode functions and @(':logic') mode functions.
+  @('Defwarrant'), on the other hand, can only analyze @(':logic') mode
+  functions because it must inspect the measure used to justify the termination
+  of the function and, if it is successful, it adds a @(':logic') mode
+  definition of the warrant to the logic.  This definition links the symbol to
+  the function via @('badge') and @('apply$') and if the warrant is a
+  hypothesis of a conjecture then the prover ``knows'' about the linkage.</p>
+
+  <p>Both @('defbadge') and @('defwarrant') affect the top-level
+  read-eval-print loop because that loop treats @(':program') and @(':logic')
+  functions differently so that it can (a) allow @(':program') mode terms to be
+  evaluated to carry out commands such as @(tsee defun) and @(tsee defthm),
+  query the world or build and test prototypes, and (b) allow @(':logic') mode
+  terms to be evaluated while guaranteeing a certain correspondence with what
+  can be proved.  See @(see guarantees-of-the-top-level-loop).</p>
 
   <h3>Requirements of @('Defbadge')</h3>
-
 
   @({
   General Form:
@@ -20958,16 +21022,17 @@ subtree of X with T, without duplication.</p>
   or @(':')@(tsee logic) mode.  This command analyzes the body of @('fn') to
   determine whether it satisfies certain stringent syntactic conditions
   discussed below.  If the conditions are not met, @('defbadge') signals an
-  error.  Otherwise, if records a @(see badge) for @('fn').  Badges record the
+  error.  Otherwise, it records a @(see badge) for @('fn').  Badges record the
   input and output arities of @('fn') and specify which arguments are
   ``functions'' that may be applied with @('apply$'), which are ``expressions''
   that may be evaluated with @(tsee ev$), and which are neither.  The
   conditions checked are sufficient to allow @(tsee apply$) to run the function
   safely at the top level of the ACL2 read-eval-print loop.  However, in order
-  to prove anything about the behavior of @('apply$') on @('fn') the function
-  will need a @(see warrant) as issued by @(tsee defwarrant).  @('Defbadge')
-  does not issue warrants, just badges.  @('Defwarrant') can issue both badges
-  and warrants.</p>
+  to prove anything about a call of @('apply$') on @('fn') &mdash; or even to
+  evaluate such a call if @('fn') is in @(':')@(tsee logic) mode, as discussed
+  above &mdash; @('fn') will need a @(see warrant) as issued by @(tsee
+  defwarrant).  @('Defbadge') does not issue warrants, just badges.
+  @('Defwarrant') can issue both badges and warrants.</p>
 
   <p>The first condition on @('fn') is that it must be a defined function
   symbol.  Since @('fn') must be defined it may not be a constrained function
@@ -20981,7 +21046,7 @@ subtree of X with T, without duplication.</p>
   <p>The other conditions depend on whether @(tsee apply$) is reachable from
   @('fn').  That is, can a call of @('fn') lead to a call of @('apply$')?  If
   @('apply$') is not reachable from @('fn'), then there are no more conditions
-  on @('fn').  A badge for fn is computed and stored.  We are more precise
+  on @('fn').  A badge for @('fn') is computed and stored.  We are more precise
   about ``reachability'' later.</p>
 
   <p>If @('apply$') is reachable from @('fn'), then there are additional
@@ -21002,14 +21067,14 @@ subtree of X with T, without duplication.</p>
   @(':EXPR')) iff it is sometimes passed into a @(':FN') (or @(':EXPR')) slot
   in the body of @('fn') and is never passed into any other kind of slot.  A
   formal can be be assigned ilk @('NIL') iff it is never passed into a slot of
-  ilk @(':FN') or @(':EXPR'), i.e., if it is used as an ``ordinary'' object.
-  We are more precise below.</p>
+  ilk @(':FN') or @(':EXPR'), i.e., if it is used exclusively as an
+  ``ordinary'' object.  We are more precise below.</p>
 
   <p><i>(b)</i> Every @(':FN') and @(':EXPR') slot of every function called in
   the body of @('fn') is occupied either by a formal of @('fn') of the same ilk
   or, in the case of calls of functions other than @('fn'), a quoted @(see
   tame) function symbol or quoted tame (preferably well-formed) @('LAMBDA')
-  object.</p>
+  object.  (See @(tsee well-formed-lambda-objectp).)</p>
 
   <p>This completes the list of restrictions imposed by @('defbadge').</p>
 
@@ -21017,14 +21082,16 @@ subtree of X with T, without duplication.</p>
 
   <p>Note that if @('apply$') is not reachable from @('fn'), the restrictions
   imposed on @('fn') are comparatively generous.  Such a @('fn') could be
-  badged despite being defined mutually recursively or in terms of unbadged or
-  even unbadgeable functions.</p>
+  badged and warranted despite being defined mutually recursively or in terms
+  of unbadged or even unbadgeable functions.  Basically, if @('fn') doesn't
+  depend on @('apply$') there is no danger that some argument of @('fn') will
+  be treated like a function object or an expression.</p>
 
   <p>After a successful @('defbadge') event for @('fn'), the function @(tsee
-  badge) will return the computed badge and @(tsee apply$) will be able to
-  accept the @('fn') as a functional argument.  Here is an annotated script.
-  First, carry out these two events, defining @('foldr') as a @(':program')
-  mode function.</p>
+  badge) will return the computed badge (when executed in the top-level loop)
+  and @(tsee apply$) will be able to accept the @('fn') as a functional
+  argument.  Here is an annotated script.  First, carry out these two events,
+  defining @('foldr') as a @(':program') mode function.</p>
 
   @({
   (include-book \"projects/apply/top\" :dir :system)
@@ -21059,12 +21126,12 @@ subtree of X with T, without duplication.</p>
   on FOLDR because FOLDR has not been badged.
   })
 
-  <p>However, we can use @('defbadge') to compute the badge for @('foldr').
-  The badge says foldr has input arity 3, output arity 1, and treats its middle
-  argument as a function.  We can recover the badge by calling the function
-  @(tsee badge).  We can successfully apply @('foldr').  We can even use it in
-  a @('lambda') expression that we pass as the middle argument to
-  @('foldr').</p>
+  <p>However, we can use @('defbadge') to compute and store the badge for
+  @('foldr').  The badge says @('foldr') has input arity 3, output arity 1, and
+  treats its middle argument as a function.  We can recover the badge by
+  calling the function @(tsee badge).  We can successfully apply @('foldr').
+  We can even use it in a @('lambda') expression that we pass as the middle
+  argument to @('foldr').</p>
 
   @({
   ACL2 !>(defbadge foldr)
@@ -21099,9 +21166,9 @@ subtree of X with T, without duplication.</p>
   warrants, we think of this test colloquially as whether @('apply$') is
   ancestral in @('fn').</p>
 
-  <p>The test and the onerous conditions imposed when the @('apply$') is
-  reachable is crucial to the soundness of the ACL2 proof theory.  We discuss
-  this further in the background material for @(tsee apply$), including <a
+  <p>The test and the onerous conditions imposed when @('apply$') is reachable
+  is crucial to the soundness of the ACL2 proof theory.  We discuss this
+  further in the background material for @(tsee apply$), including <a
   href='http://www.cs.utexas.edu/users/kaufmann/papers/apply/index.html'>``Limited
   Second-Order Functionality in a First-Order Setting''</a> by Matt Kaufmann
   and J Strother Moore and offer a fully fleshed out metalevel proof that
@@ -21109,10 +21176,11 @@ subtree of X with T, without duplication.</p>
   titled <tt>Essay on Admitting a Model for Apply$ and the Functions that Use
   It</tt> in the ACL2 source file @('apply-raw.lisp').</p>
 
-  <p>But badges are more concerned with the evaluation theory than the proof
-  theory.  Even if we convert @('foldr') to @(':logic') mode we cannot prove
-  anything interesting about what happens when it is applied with
-  @('apply$').</p>
+  <p>But badges are more concerned with syntax (and, for @(':program') mode
+  functions, evaluation) than the proof theory.  Even if we convert @('foldr')
+  to @(':logic') mode we cannot prove anything interesting about what happens
+  when it is applied with @('apply$').  We can't even prove that @('foldr') has
+  a badge or what that badge is!</p>
 
   @({
   ACL2 !>(verify-termination foldr)
@@ -21124,10 +21192,19 @@ subtree of X with T, without duplication.</p>
                   (append x z)))
   [Unsuccessful.  Output deleted.]
   ******** FAILED ********
+
+  ACL2 !>(thm
+           (equal (badge 'foldr) '(APPLY$-BADGE 3 1 NIL :FN NIL)))
+  [Unsuccessful.  Output deleted.]
+  ******** FAILED ********
+
   })
 
-  <p>In order to prove anything about applying @('foldr') we need the @(tsee
-  warrant) for @('foldr').  Warrants are issued by @(tsee defwarrant).</p>
+  <p>In order to prove anything nontrivial about @('foldr')'s badge or behavior
+  under @('apply$') we need the @(tsee warrant) for @('foldr').  Warrants are
+  issued by @(tsee defwarrant).  If we execute (defwarrant foldr) and then
+  amend the failed @('thm') commands above by adding @('(warrant foldr)') as a
+  hypothesis, both amended formulas are provable.</p>
 
   <h3>How Ilks Are Assigned</h3>
 
@@ -21144,10 +21221,13 @@ subtree of X with T, without duplication.</p>
   @('fn') is warranted.</p>
 
   <p>The key to the inductive correctness of the algorithm implicity described
-  below is the fact that initially the only function symbol with a slot of ilk
-  @(':FN') is @('apply$') and the only function with a slot of ilk @(':EXPR')
-  is @('ev$').  In both functions it is the first argument slot that is so
-  distinguished.</p>
+  below is the fact that when the ACL2 logic is being booted up the only
+  function symbol with a slot of ilk @(':FN') is @('apply$') and the only
+  function with a slot of ilk @(':EXPR') is @('ev$').  In both functions it is
+  the first argument slot that is so distinguished.  All other ACL2 primitives
+  that use @('apply$') or @('ev$'), e.g., @('collect$'), are defined,
+  admissible, badged, and warranted under the same conditions user-defined
+  functions are.</p>
 
   <p>Let <i>v </i> be the <i>i </i>th formal parameter of a defined function
   <i>fn</i>.  Then the ilk of <i>v </i> is @(':FN') iff the value of <i>v </i>
@@ -25869,23 +25949,9 @@ subtree of X with T, without duplication.</p>
 
   <h3>Badges versus Warrants</h3>
 
-  <p>It is easy to confuse badges, which are issued by @(tsee defbadge), with
-  warrants, which are issued by @('defwarrant').  The thing to keep in mind is
-  that badges extend the syntax and evaluation capabilities of ACL2, while
-  warrants extend the proof theory.  Some user-defined function symbols may be
-  given badges even if they are in @(':')@(tsee program) mode (see @(see
-  mixed-mode-functions)).  If @('fn') has a badge, you are allowed to write
-  @('(apply$ 'fn (list a1 ... an))') and expect it evaluate ``correctly'' at
-  the top level of the ACL2 read-eval-print loop, just as you expect @('(fn a1
-  ... an)') to evaluate.  But you cannot <i>prove</i> anything interesting
-  about @('(apply$ 'fn (list a1 ... an))') without the warrant for @('fn').  A
-  badged but unwarranted function symbol might as well be undefined as far as
-  the prover is concerned.  Warrants connect the quoted symbol to the axiomatic
-  behavior of @('apply$'), in particular, they constrain @('(apply$ 'fn (list
-  a1 ... an))') to be @('(fn a1 ... an)') under certain conditions.  Obviously,
-  the very first requirement on @('fn') to have a warrant is that @('fn') must
-  be in @(':')@(tsee logic) mode.  But there are other requirements because
-  @('defwarrant') must make sure the extended proof theory is consistent.</p>
+  <p>It is easy to confuse @(see badge)s, which are issued by @(tsee defbadge),
+  with @(see warrant)s, which are issued by @('defwarrant').  See the first
+  section of @(tsee defbadge) for an extended discussion.</p>
 
   <h3>Requirements of @('Defwarrant')</h3>
 
@@ -25898,11 +25964,11 @@ subtree of X with T, without duplication.</p>
   of @('fn') to determine whether it satisfies certain stringent syntactic and
   semantic conditions that allow the ACL2 proof theory to be extended so that
   the prover can simplify forms like @('(apply$ 'fn ...)').  The syntactic
-  conditions are actually those of @(tsee defbadge), which @('defwarrant')
-  essentially invokes if @('fn') is not already badged.  But below we describe
-  all the conditions &mdash; those enforced by @('defbadge') and those unique
-  to @('defwarrant') &mdash; since many users use @('defwarrant') to issue both
-  a badge and a warrant.</p>
+  conditions include those of @(tsee defbadge), which @('defwarrant')
+  essentially invokes if @('fn') is a @(':')@(tsee logic) mode function that is
+  not already badged.  But below we describe all the conditions checked by
+  @('defwarrant') since many users use @('defwarrant') to issue both a badge
+  and a warrant.</p>
 
   <p>Basic conditions include that @('fn') is in @(':')@(tsee logic)-mode and
   that its justification (i.e., the measure, well-founded relation, and domain
@@ -25926,11 +25992,12 @@ subtree of X with T, without duplication.</p>
   function in the Community Books at @('books/ordinals/').</p>
 
   <p><i>(b)</i> Every function called in the body of @('fn'), except @('fn')
-  itself, must already have a @(see badge).  If some subfunction doesn't
-  already have a badge, @('defwarrant') will signal an error and report the
-  unbadged function.  You will have to call @('defwarrant') on that function
-  &mdash; and that call must succeed &mdash; before any function using it is
-  successfully warranted.</p>
+  itself, must already have a @(see badge) and a warrant.  If some subfunction
+  doesn't already have a badge, @('defwarrant') will call @(tsee defbadge) and
+  signal an error if that fails.  If some subfunction doesn't already have a
+  warrant, @('defwarrant') will signal an error and suggest that you call
+  @('defwarrant') on the offending subfunction first.  @('Defwarrant') will
+  continue to fail until all subfunctions have badges and warrants.</p>
 
   <p><i>(c)</i> It must be possible for each formal of @('fn') to be assigned
   one of three @(see ilk)s, @(':FN'), @(':EXPR'), or @('NIL'), as described
@@ -25961,7 +26028,14 @@ subtree of X with T, without duplication.</p>
   cannot be reached are comparatively generous.  If @('fn') does not depend on
   @('apply$') then @('fn') can be warranted despite (a) being defined mutually
   recursively or with an arbitrary ordinal measure, or (b) calling unbadged or
-  unbadgeable functions.</p>
+  unbadgeable functions.  @('Defwarrant') can be relaxed in this case because
+  the warrant constrains @('(apply$ 'fn ...)') to be @('(fn ...)') and @('fn')
+  is a well-defined @(':logic') mode function that is independent of
+  @('apply$').  Thus, in the model of @('apply$') that justifies the whole
+  @('apply$') story, the handling of @('fn') is just a base case.  The
+  situation would be more restrictive if the warrant constrained @('(apply$ 'fn
+  ...)') to evaluate the body of @('fn') with @(tsee ev$) which would possibly
+  raise termination issues.</p>
 
   <p>Regardless of whether @('apply$') is reachable, if the requisite
   conditions are not met, @('defwarrant') causes an error.</p>
@@ -27187,10 +27261,10 @@ ld) and @(tsee include-book)"
  </ul>
 
  <p>Notice that in code, where restrictions on return values are in force, no
- stobj may be let-bound in a DO body or FINALLY clause.  This is due not only
- to the explicit restriction above for @('LET'), @('LET*'), and @('MV-LET')
- expressions, but also due to the first condition above, on ordinary terms
- returning a single, non-stobj value.</p>
+ stobj may be let-bound in a @('DO') body or @('FINALLY') clause.  This is due
+ not only to the explicit restriction above for @('LET'), @('LET*'), and
+ @('MV-LET') expressions, but also due to the first condition above, on
+ ordinary terms returning a single, non-stobj value.</p>
 
  <p>We conclude this section by discussing some syntactic restrictions.</p>
 
@@ -35104,7 +35178,7 @@ current fast alists."
 
   <p>Notice the addition of hypotheses above of the form @('(warrant ...)').
   ACL2 adds such <i>@(see warrant) hypotheses</i> for function symbols that
-  might be @(tsee apply$)ed during evaluation of a scion call (in this case,
+  might be @(tsee apply$)'d during evaluation of a scion call (in this case,
   @('sum$')).</p>
 
   <p>In general, you may notice that ACL2 generates such ``special'' guard
@@ -39919,6 +39993,546 @@ current fast alists."
  an <i>untranslated</i> term, that is, a user-level term; see @(see term).
  The corresponding call @('(guard-theorem x simplify guard-debug (w state)
  state)') returns a translated term.</p>")
+
+(defxdoc guarantees-of-the-top-level-loop
+  :parents (ld)
+  :short "ACL2 interactive top-level read-eval-print loop"
+  :long "<p>We often refer to the ``top-level loop,'' or just ``the loop'' when
+  the context is understood.  The loop is the interactive read-eval-print loop
+  with which the user interacts to issue commands, query the ACL2 logical
+  world, test functions, conjectures, and systems, etc.  This documentation
+  topic mainly addresses the logical guarantees of the loop.  For practical
+  advice about interacting with and configuring the loop see @(tsee ld).
+  @('Ld') is the ACL2 implementation of the loop (as a macro that calls a
+  @(tsee state)-using function with many parameters which may be set by the
+  user).  @('Ld') is called initially when ACL2 is fired up.</p>
+
+  <p>But here we are concerned with what it means, logically, when a term
+  <i>tm</i> evaluates without error to a value <i>v</i> in the loop.</p>
+
+  <h3>A Strawman Proposal on the Meaning of Top-Level Evaluation</h3>
+
+  <p>One might like to think that for any term, <i>tm</i>, a non-erroneous
+  interaction like</p>
+
+  <code>
+  ACL2 !&gt;<i>tm</i>
+  <i>v</i>
+  </code>
+
+  <p>means that the formula</p>
+
+  <code>
+  (equal <i>tm</i> '<i>v</i>)
+  </code>
+
+  <p>is a theorem and can be proved by the prover.</p>
+
+  <p>For example, let @('sq') be a :logic mode function that squares its
+  argument.  (For the sake of a later example, let us also make the @(see
+  guard) of @('sq') be @('t') and verify the guard by fixing (with @(tsee
+  rfix)) the argument to be a rational, but those aspects of @('sq') are
+  irrelevant in our immediate use of it below.)</p>
+
+  <code>
+  (defun sq (x)
+    (declare (xargs :guard t :verify-guards t))
+    (let ((x (rfix x)))
+      (* x x)))
+  </code>
+
+  <p>then the evaluation</p>
+
+  <code>
+  ACL2 !&gt;(sq 3)
+  9
+  </code>
+
+  <p>suggests that @('(equal (sq 3) 9)') is a theorem and that is indeed
+  provable by the ACL2 theorem prover.</p>
+
+  <p>But the situation is quite subtle and deserves further discussion.  That
+  is what this topic is about.</p>
+
+  <p><b>Spoiler Alert</b>: We will not give logical semantics to every
+  non-erroneous evaluation in this discussion.  We only hint at how it can be
+  done for many terms.  Furthermore, even for those terms whose evaluations do
+  correspond to theorems, the logical theory in which those theorems can be
+  proved is not the theory supported by the ACL2 prover but an extension of it.
+  We ultimately describe below the so-called <i>evaluation theory</i> which is
+  an extension of ACL2's <i>proof theory</i>.  So this documentation topic
+  discusses two logical theories.  Because any theory in which proofs are done
+  might be called the ``proof theory'' and in this section we need to clearly
+  distinguish between the two theories being discussed, we'll refer to the
+  theory supported by the ACL2 theorem prover as the <i>prover's
+  theory</i>.</p>
+
+  <h3>Problems Raised by @(':Program') Mode Functions</h3>
+
+  <p>Suppose @('prog-sq') is defined as a @(':')@(tsee program) mode function
+  that squares its argument.  Then the top-level evaluation</p>
+
+  <code>
+  ACL2 !&gt;(prog-sq 3)
+  9
+  </code>
+
+  <p>clearly should not suggest</p>
+
+  <code>
+  (equal (prog-sq 3) 9)
+  </code>
+
+  <p>is a theorem.  @(':Program') mode functions are not defined in the
+  prover's theory.  (@(':Program') mode functions may not terminate and any
+  naive attempt to add their definitions to the prover's theory as axioms could
+  result in unsoundness.)  The top-level loop has the ability to evaluate
+  @(':program') mode expressions but it is ``magic,'' unsupported by proof.
+  (Non-termination by the evaluator can't manifest unsoundness: such
+  computations just never produce an answer.)  The evaluation of @(':program')
+  mode expressions is supported in the loop primarily as a way to execute
+  commands like @(tsee defun) and @(tsee defthm).  But it is also a convenience
+  that allows ACL2 to be used as a @(see programming) language (e.g., to
+  prototype a system one might eventually admit to the logic and prove theorems
+  about).</p>
+
+  <p>Therefore, when attempting to define the logical meaning of top-level
+  evaluations we might restrict our attention to @(':')@(tsee logic) mode terms
+  only.  But this is not sufficient for several reasons.</p>
+
+  <p>@(':Program') mode functions raise another problem discussed below in
+  connection with @('apply$').</p>
+
+  <h3>Problems Raised by Single-Threaded Objects</h3>
+
+  <p>Evaluation of terms involving single-threaded objects or ``@(see stobj)s''
+  raise problems, even if the terms involved are in @(':logic') mode.  Here is
+  a top-level evaluation sequence</p>
+
+  <code>
+  ACL2 !&gt;(defstobj st fld)
+  ...
+  ST
+  ACL2 !&gt;(update-fld 3 st)
+  &lt;st&gt;
+  ACL2 !&gt;(update-fld (sq (fld st)) st)
+  &lt;st&gt;
+  ACL2 !&gt;(fld st)
+  9
+  </code>
+
+  <p>but the strawman conjecture from the last evaluation, @('(equal (fld st)
+  9)'), is not a theorem.  However, a related formula is a theorem and can be
+  proved by the prover.</p>
+
+  <code>
+  (implies (stp st)
+           (let* ((st (update-fld 3 st))
+                  (st (update-fld (sq (fld st)) st)))
+             (equal (fld st) 3)))
+  </code>
+
+  <p>This reminds us that the top-level loop tracks changes to each ``live''
+  stobj and records them in the ACL2 @(tsee state).  Those changes must be
+  reflected in any suggested theorems.</p>
+
+  <h3>Problems Raised by Apply$</h3>
+
+  <p>@(tsee Apply$) calls @(tsee apply$-userfn) to handle the application of
+  user-defined function symbols.  @('Apply$-userfn') is undefined but might be
+  constrained by @(tsee warrant) hypotheses (see @(tsee defwarrant)).  Recall
+  that warrants link the functions approved by @('defwarrant') to their names
+  and constrain @('(apply$ 'fn (list a1 ... an))') to be @('(fn a1 ... an)')
+  under certain @(tsee tame)ness conditions.  As noted at the bottom of the
+  discussion of @(tsee defwarrant), there is a model of the prover's theory in
+  which all warrants issued by @('defwarrant') are true.  The top-level loop
+  assumes that all those warrants are true.  But the prover's theory does not,
+  because explicit warrant hypotheses are essential to avoiding the so-called
+  ``local problem'' (see <b>Lesson 12</b> of @(see
+  introduction-to-apply$)).</p>
+
+  <p>One might wonder why we have warrants at all, aside from the local
+  problem.  The key reason is that inconsistency can result from
+  non-terminating recursion if we had the following
+  axiom schema</p>
+
+  <code>
+  <b>Unsound Axiom Schema</b>:
+  (equal (apply$ '<i>f</i> (list a1 ... an)) (<i>f</i> a1 ... an))
+  </code>
+
+  <p>for every defined function <i>f</i>.  See the @('russell') example in
+  @(see introduction-to-apply$).  So warrants and the restrictions enforced by
+  @(tsee defwarrant) keep the prover's theory consistent.  One might then ask
+  ``how do we get away with letting the top-level loop @('apply$') all badged
+  @(':program') mode functions?''  The answer is simple: @(':program') mode
+  functions are not axiomatized so we don't have a theory to worry about!</p>
+
+  <p>To illustrate the difference between the behavior of the top-level loop
+  and the prover, suppose the function @('sq'), defined above, has been
+  warranted.</p>
+
+  <code>
+  (defwarrant sq)
+  </code>
+
+  <p>and then consider the top-level evaluation</p>
+
+  <code>
+  ACL2 !&gt;(apply$ 'sq '(3))
+  9
+  </code>
+
+  <p>This is possible because the warrant for @('sq') is assumed true in the
+  top-level loop and that warrant tells the loop that @('(apply$ 'sq '(3))') =
+  @('(sq 3)').</p>
+
+  <p>However, @('(equal (apply$ 'sq '(3)) '9)') is not a theorem in the
+  prover's theory.  Instead, this is a theorem</p>
+
+  <code>
+  (implies (warrant sq)
+           (equal (apply$ 'sq '(3)) '9))
+  </code>
+
+  <p>where @('(warrant sq)') is just a convenient abbreviation for
+  @('(apply$-warrant-sq)').</p>
+
+  <p>Thus, to extend the strawman conjecture to functions in which @('apply$')
+  is ancestral would require tracking the warrants relevant to the execution
+  path (or punting and collecting all warrants) and amending the conjecture to
+  add those warrants as hypotheses to the equality.</p>
+
+  <p>But @('apply$') introduces another source of complexity: mixed-mode
+  functions (see @(see mixed-mode-functions)).  Recall the @(':program') mode
+  function @('prog-sq') which squares its argument.  We can assign a badge to
+  @('prog-sq') and then define a @(':logic') mode function that @('apply$')s
+  it!</p>
+
+  <code>
+  (defbadge prog-sq)
+
+  (defun logic-sq (x)
+    (declare (xargs :mode :logic))
+    (apply$ 'prog-sq (list x)))
+  </code>
+
+  <p>Since the top-level loop can evaluate applications of @(':program') mode
+  symbols we see the following evaluation.</p>
+
+  <code>
+  ACL2 !&gt;(logic-sq 3)
+  9
+  </code>
+
+  <p>Note that @('(logic-sq 3)') is a @(':logic') mode term and @('logic-sq')
+  can even be warranted with @('defwarrant').  But neither</p>
+
+  <code>
+  (equal (logic-sq 3) '9)
+  </code>
+
+  <p>nor</p>
+
+  <code>
+  (implies (warrant logic-sq) (equal (logic-sq 3) '9))
+  </code>
+
+  <p>is a theorem in the prover's theory because @('prog-sq') is undefined in
+  that theory.  For what it is worth, the prover can prove</p>
+
+  <code>
+  (implies (warrant logic-sq) (equal (logic-sq 3) (apply$ 'prog-sq '(3))))
+  </code>
+
+  <p>This example contradicts the suggestion, just above, that if we properly
+  considered warrants we could give logical meaning to evaluations of
+  @(':logic') mode terms involving @('apply$').</p>
+
+  <h3>Problems Raised by Constrained Functions</h3>
+
+  <p>Constrained functions raise problems if they have been given
+  attachments (see @(tsee defattach)).  The top-level loop uses attachments to
+  compute values consistent with the constraints, but the prover's theory does
+  not.  Attachments are useful for building and testing instances of models
+  consistent with the constraints.</p>
+
+  <p>For example, let @('(nonneg-rat x)') be constrained to return some
+  nonnegative rational.</p>
+
+  <code>
+  (encapsulate (((nonneg-rat *) =&gt; *))
+    (local (defun nonneg-rat (x)
+             (declare (ignore x))
+             0))
+    (defthm nonneg-rat-constraint
+      (and (rationalp (nonneg-rat x))
+           (&lt;= 0 (nonneg-rat x)))))
+  </code>
+
+  <p>It is impossible to evaluate @('(nonneg-rat 3)') in the top-level loop.
+  But we can attach another function to it provided we can prove that function
+  always returns a nonnegative rational.  Since @('sq'), as defined above to
+  @('rfix') its argument as a rational, satisfies that constraint, we can attach
+  @('sq') to @('nonneg-rat').</p>
+
+  <code>
+  (defattach nonneg-rat sq)
+  </code>
+
+  <p>and then we can ``evaluate'' calls of @('nonneg-rat') in the loop, getting
+  results that are consistent with its constraint (but overly specific!).</p>
+
+  <code>
+  ACL2 !&gt;(nonneg-rat 3)
+  9
+  </code>
+
+  <p>But of course the strawman conjecture @('(equal (nonneg-rat 3) '9)') is
+  not a theorem of the prover's theory.</p>
+
+  <h3>The Prover's Theory</h3>
+
+  <p>The ACL2 logic formalizes an applicative (functional and side-effect free)
+  extension of a subset of Common Lisp (see @(see common-lisp)).  It is
+  described in chapter 6 of <a
+  href='http://www.cs.utexas.edu/users/moore/publications/acl2-books/car/index.html'>Computer-Aided
+  Reasoning: An Approach</a>, by Kaufmann, Manolios, and Moore, as an extension
+  of quantifier-free first-order logic with equality (section 6.1).  The syntax
+  is that of translated @(see term)s though the user is allowed to use a more
+  flexible syntax which can be extended by defining constant symbols and
+  macros (see @(tsee defconst) and @(tsee defmacro)).  To see the formal
+  translation of such a term use the command @(':')@(tsee trans).  In section
+  6.2 of the book, axioms are added to characterize the basic data objects of
+  numbers (integers, rationals, and complex rationals), characters, strings,
+  symbols, and ordered pairs.  In section 6.3, the ordinals up to epsilon-0 are
+  constructed from ordered pairs and integers; a well-founded ``less than''
+  relation is also defined.  But the book's construction of the ordinals is now
+  obsolete.  A new representation was implemented after the book was published.
+  See @(see ordinals).  In Section 6.4, a conservative Principle of
+  Definition (see @(tsee defun) and @(tsee defuns) or @(tsee mutual-recursion))
+  is introduced, allowing the addition of axioms defining new function symbols.
+  In Section 6.5, a Principle of Induction up to epsilon-0 is described.
+  Induction and recursion are duals: every admissible recursive function
+  suggests an induction and vice versa and this duality is used by the ACL2
+  prover to select an often appropriate induction scheme for a conjecture.  See
+  @(see induction) and @(tsee hints) for ways to influence this selection.
+  Finally, in section 6.6, the book introduces @(tsee encapsulate) to introduce
+  constrained functions and functional instantiation (a derived rule of
+  inference akin to second order instantiation), and a variety of other ways of
+  conservatively adding new function symbols.</p>
+
+  <p>The ACl2 prover proves theorems in the extension of the above theory
+  obtained by adding the axioms introduced by @(see events) successfully
+  carried out in the user's session.  The most common such axiom-adding events
+  are @(tsee defun), @(tsee defchoose), and @(tsee encapsulate), which all
+  conservatively extend the theory by the addition of axioms about new function
+  symbols.  But @('defun') is just a special case of @('defuns') which adds a
+  mutually recursive clique of new names (see also @(tsee mutual-recursion)).
+  @(tsee Defstobj) and @(tsee defabsstobj) add recognizers, constructors, and
+  accessors for single-threaded objects (aka ``@(see stobj)s'') but logically
+  just use @('defun') to add new functions and then syntactically restrict
+  their use.  Finally, we provide a means of adding an arbitrary formula as an
+  axiom, @(tsee defaxiom), but <i>strongly discourage its use</i>.  There are
+  many other events that add axioms, e.g., @(tsee defun-nx) and @(tsee
+  defun-sk) but these are defined as macros that expand into the primitives
+  just listed.  In addition, there is a facility for including files of
+  previously admitted events, @(tsee include-book).</p>
+
+  <p>Given a user's session, we call the above described theory the <i>prover's
+  theory</i>.</p>
+
+  <p>Now recall the strawman proposal for what evaluation in the top-level loop
+  means, i.e., that the evaluation</p>
+
+  <code>
+  ACL2 !&gt;<i>tm</i>
+  <i>v</i>
+  </code>
+
+  <p>might mean that the formula</p>
+
+  <code>
+  (equal <i>tm</i> '<i>v</i>)
+  </code>
+
+  <p>is a theorem.  We have illustrated with @(':program') mode functions, uses
+  of @('apply$'), and of constrained functions that this strawman conjecture is
+  <i>not</i> necessarily a theorem of the prover's theory!</p>
+
+  <p>However, there is a theory in which many of these conjectures are
+  theorems.</p>
+
+  <h3>The Evaluation Theory</h3>
+
+  <p>The <i>evaluation theory</i> is obtained from the prover's theory as
+  follows.</p>
+
+  <ul>
+
+  <li><p>Instead of treating stobj names as variables, the evaluation theory
+p  treats them as abbreviations for the ``current value'' of the stobj,
+  specifically, the constant obtained by composing the sequence of all updates
+  to the stobj's fields carried out so far in the top-level loop.  Thus, for
+  example, in the evaluation theories created by this sequence of top-level
+  evaluations</p>
+
+  <code>
+  ACL2 !&gt;(defstobj st fld)                           ; [1]
+  ST
+  ACL2 !&gt;(update-fld 3 st)                           ; [2]
+  &lt;st&gt;
+  ACL2 !&gt;(update-fld (* (fld st) (fld st)) st)       ; [3]
+  &lt;st&gt;
+  </code>
+
+  <p>@('st') is an abbreviation for @('(NIL)') after evaluation [1], an
+  abbreviation for @('(3)') after evaluation [2], and an abbreviation for
+  @('(9)') after evaluation [3].</p></li>
+
+  <li><p>Every warrant created by @('defwarrant') is assumed true as an
+  axiom.</p></li>
+
+  <li><p>For every @('(defattach f g)') event in the prover's theory the
+  axiom (i.e., constraints) on @('f') is replaced by the axiom @('(equal (f
+  ...) (g ...))') in the evaluation theory.</p></li>
+
+  </ul>
+
+  <p>Given the restrictions enforced by @('defun'), @('defstobj'),
+  @('defwarrant'), @('apply$'), @('encapsulate'), and @('defattach'), the
+  evaluation theory is consistent if the prover's theory is consistent and free
+  of @('defaxiom') events.</p>
+
+  <p>Furthermore, the top-level evaluation</p>
+
+  <code>
+  ACL2 !&gt;<i>tm</i>
+  <i>v</i>
+  </code>
+
+  <p>means that</p>
+
+  <code>
+  (equal <i>tm</i> '<i>v</i>)
+  </code>
+
+  <p>is a theorem in the evaluation theory provided</p>
+
+  <ul>
+
+  <li><i>tm</i> is a @(':logic') mode term, and</li>
+
+  <li>every symbol that reaches the first argument of any @('apply$-userfn') in
+  the execution of <i>tm</i> is in @(':logic') mode.</li>
+
+  </ul>
+
+  <p>The ACL2 prover cannot generally prove these theorems, since it operates
+  in the prover's theory.  However, as noted, there are often ways to encode
+  the conjectures into ACL2 formulas that are provable though the ACL2 system
+  does not provide tools for doing so.</p>
+
+  <h3>Some Examples of Top-Level Evaluations</h3>
+
+  <p>In this section we illustrate some consequences of the guarantee that for
+  any term, <i>tm</i>, satisfying certain restrictions, if <i>tm</i> evaluates
+  to a value <i>v</i>, then the term</p>
+
+  <code>
+  (equal <i>tm</i> '<i>v</i>)
+  </code>
+
+  <p>is a theorem of the evaluation theory.</p>
+
+  <p>Each command below is enumerated and after the entire sequence we make
+  observations about the results and implications.  It might also help to read
+  the section <b>Top-Level Evaluation of Apply$</b> in the documentation for
+  @(tsee apply$), which describes how @('apply$') is implemented in the
+  top-level loop.</p>
+
+  @({
+  ACL2 !>(include-book \"projects/apply/top\" :dir :system)
+  ...
+  ACL2 !>(defun my-cons (x y)                                  ; [1]
+            (declare (xargs :mode :program))
+            (cons x y))
+  ...
+  ACL2 !>(defbadge my-cons)                                    ; [2]
+
+  MY-CONS now has the badge (APPLY$-BADGE 2 1 . T) but has
+  no warrant.
+
+   T
+  ACL2 !>(apply$ 'my-cons '(3 4))                              ; [3]
+  (3 . 4)
+  ACL2 !>(thm (equal (my-cons 3 4) '(3 . 4)))                  ; [4]
+  ...
+  ******** FAILED ********
+  ACL2 !>(verify-termination my-cons)                          ; [5]
+  ...
+  ACL2 !>(apply$ 'my-cons '(3 4))                              ; [6]
+
+
+  ACL2 Error in TOP-LEVEL:  The value of APPLY$-USERFN is not
+   specified on MY-CONS because MY-CONS has not been warranted.
+
+  ACL2 !>(defwarrant my-cons)                                  ; [7]
+
+  MY-CONS is now warranted by APPLY$-WARRANT-MY-CONS, with
+  badge (APPLY$-BADGE 2 1 . T).
+
+  ACL2 !>(apply$ 'my-cons '(3 4))                              ; [8]
+  (3 . 4)
+
+  ACL2 !>ACL2 !>(thm (equal (my-cons 3 4) '(3 . 4)))           ; [9]
+  ...
+  ******** FAILED ********
+  ACL2 !>(thm                                                  ;[10]
+          (implies (warrant my-cons)
+                   (equal (my-cons 3 4) '(3 . 4))))
+  ...
+  Q.E.D.
+  ...
+  Proof succeeded.
+  })
+
+  <p>In events [1] and [2] @('my-cons') is introduced as a badged @(':program')
+  mode function.  Command [3] shows that we can @('apply$') @(''my-cons') in
+  the top-level loop and get the ``expected'' value.  This is ``magic'' on
+  several levels!  There is no axiom in the evaluation theory defining
+  @('my-cons') and there is no warrant connecting the symbol @(''my-cons') to
+  the function @('my-cons').  The failure of the first @('thm') command, [4],
+  shows that the prover's theory knows nothing of the behavior of @('apply$')
+  on @(''my-cons').  After converting @('my-cons') to @(':logic') mode with
+  @(tsee verify-termination) in [5] we can no longer evaluate the application
+  of @('my-cons') at the top-level, as shown by [6]!  This is surprising
+  because one might expect ACL2 to be able to do more with a @(':logic') mode
+  function than its @(':program') mode counterpart.  But in the evolving
+  evaluation theory as of [6], @('my-cons') is a @(':logic') mode function with
+  no warrant and so logically speaking @('(apply$ 'my-cons ...)')  is
+  undefined.  Computing a value for it at [6] would violate the guarantee that
+  values of @(':logic') mode terms can be proved correct in the evaluation
+  theory &mdash; i.e., that the computed value can be derived logically.  Such
+  a derivation is impossible without a warrant.  However, after
+  @('defwarrant'), in [7], confirms that it is sound to issue a
+  warrant (linking the symbol @(''my-cons') to the function @('my-cons') via
+  @('apply$')), the evaluation of the @(''my-cons') term in [8] succeeds.  The
+  @('defwarrant') soundly extends the proof theory by adding a definition for
+  the warrant function for @('my-cons') and extends the evaluation theory by
+  assuming the warrant for @('my-cons') is true.  This latter extension is also
+  sound.  However, [9] shows that we still cannot prove (in the prover's
+  theory) that the evaluation of the @('apply$') term is correct, because we
+  did not provide the warrant as a hypothesis.  However, if we amend the
+  conjecture to include the warrant, as in [10], the proof (in the prover's
+  theory) succeeds.  While all warrants are assumed true in the evaluation
+  theory, they must be made explicit as hypotheses for proofs in the prover's
+  theory.  This is the mechanism whereby ACL2 can avoid the ``local problem''
+  illustrated <b>Lesson 12</b> of @(see introduction-to-apply$) and discussed
+  more thoroughly in <a
+  href='http://www.cs.utexas.edu/users/kaufmann/papers/apply/index.html'>``Limited
+  Second-Order Functionality in a First-Order Setting''</a> by Matt Kaufmann
+  and J Strother Moore.</p>")
 
 (defxdoc guard
   :parents (programming xargs)
@@ -51813,7 +52427,7 @@ tables in the current Hons Space."
   <i>become</i> ill-formed by an undo.  So at runtime @('apply$') has to check
   that the function symbol or @('LAMBDA') object is appropriate.  There is a
   sophisticated cache behind the execution machinery for @('LAMBDA') objects in
-  the evaluation theory.</p>
+  the evaluation theory.  See @(tsee print-cl-cache).</p>
 
   <h3>About Lambda$ Expressions</h3>
 
@@ -56333,13 +56947,18 @@ forms allowed for a @('let') form are  @('ignore'), @('ignorable'), and
  <li><b>Many examples</b> of @(tsee loop$) expressions may be found in @(see
  community-book) @('projects/apply/loop-tests.lisp').</li>
 
- <li>Before using @('loop$'), it is <b>strongly recommended</b> that you
- include the same book as is typically included when using @(tsee apply$), as
- follows.
+ <li>The semantics of @('loop$') involve @('apply$').  Therefore, before using
+ @('loop$'), it is <b>strongly recommended</b> that you include the same book
+ as is typically included when using @(tsee apply$), as follows.
 
  @({
  (include-book \"projects/apply/top\" :dir :system)
  })</li>
+
+ <li>ACL2 @('loop$') statements are executed as Common Lisp @('loop')
+ statements after the relevant @(see guard) conjectures are proved.  Common
+ Lisp @('loop') statements generally execute much faster than
+ equivalent (tail-recursive) functions.</li>
 
  <li><b>Warning:</b> @('Loop$') implements only a modest part of the
  functionality of Common Lisp's @('loop').  Aside from the simple fact that
@@ -56401,11 +57020,11 @@ forms allowed for a @('let') form are  @('ignore'), @('ignorable'), and
  certain places and these are ignored by Common Lisp.</p>
 
  <p>Next we present some @('FOR') @('loop$') examples.  They illustrate the
- three supported forms of iteration: the use of @('IN'), to iterate over
- elements of a list; the use of @('ON'), to iterate over the non-empty tails of
- a list; and the use of @('FROM .. TO'), to iterate over a range of
- integers (optionally with @('BY') to specify the increment at each step).
- These examples also illustrate the use of @('WHEN') to restrict which
+ three supported forms of @('FOR') @('loop$') iteration: the use of @('IN'), to
+ iterate over elements of a list; the use of @('ON'), to iterate over the
+ non-empty tails of a list; and the use of @('FROM .. TO'), to iterate over a
+ range of integers (optionally with @('BY') to specify the increment at each
+ step).  These examples also illustrate the use of @('WHEN') to restrict which
  iterations are considered and the use of @('UNTIL') to terminate early.
  Additional keywords illustrated are @('OF-TYPE') to specify types and @('AS')
  to specify additional iteration variables.  They also illustrate some of the
@@ -56477,12 +57096,27 @@ forms allowed for a @('let') form are  @('ignore'), @('ignorable'), and
  @(':VALUES') keyword specifies the shape of the return.  We also see here the
  use of the optional @(':GUARD') keyword of a @('loop$') expression (legal for
  both classes of @('loop$')s, as discussed further below) and the optional
- @(':MEASURE') keyword of a @('DO') @('loop$') expression.  Notice the @(tsee
- defwarrant) events: for a @(see guard)-verified function, warrants are
- necessary for non-built-in functions called in the body of any @('loop$')
- expression, in the @('FINALLY') clause of a @('DO') @('loop$'), or in the
- @('UNTIL') or @('WHEN') test of a @('FOR') @('loop$') expression.  @(csee
- Badge)s suffice in place of warrants if guards are not verified.</p>
+ @(':MEASURE') keyword of a @('DO') @('loop$') expression.</p>
+
+ <p>But notice the @(tsee defwarrant) events below!  They are required because
+ the functions @('fld') and @('update-fld') are not system primitives.  They
+ are introduced by the user's @(tsee defstobj) event below.  This is in
+ contrast to the @('DO') @('loop$') in our first example above where no
+ warrants are required because all the functions in that example are
+ primitive.</p>
+
+ <p>The semantics of @('loop$') involve @('apply$') and thus @('loop$')s
+ inherit the restrictions imposed on @('apply$') and its @(see scion)s.  Among
+ those restrictions are that (a) unwarranted @(':logic') mode functions cannot
+ be @('apply$')'d in the top-level read-eval-print loop and (b) proofs about
+ the applications of unwarranted functions are impossible.  Restriction (a)
+ means you cannot even execute a @(':logic') mode @('loop$') containing
+ unwarranted functions.  Restriction (b) means you can't verify the @(see
+ guard)s of such @('loop$').  This last point obviates the main reason for
+ using @('loop$'): its fast execution as a Common Lisp loop once guards are
+ verified.</p>
+
+ <p>Now here is our second example.</p>
 
  @({
 
@@ -56521,18 +57155,25 @@ forms allowed for a @('let') form are  @('ignore'), @('ignorable'), and
 
  <p>Both classes of @('loop$') expressions (@('FOR') and @('DO') @('loop$')s)
  rely heavily on the ACL2 built-in function, @(tsee apply$): in each iteration
- through the loop, a @(see lambda) object based on the body of the loop is
- given as the function argument of @('apply$').  Because of this, and because
- the value returned by @('apply$') is unspecified in the absence of @(see
- warrant)s for relevant user-defined function symbols, such warrants are needed
- for reasoning about @('loop$') expressions as well.  The documentation for
- @(tsee apply$) illustrates a simple @('defun') that is inadmissible because
- the measure theorem cannot be proved without a warrant and warrants cannot be
- assumed during the proofs of the measure conjectures.  The same issue arises
- when one of the functions critically involved in a measure conjecture is
- defined using a @('loop$') whose body involves a user-defined function.  For a
- simple example of this issue and how to work around it, see @(see
- community-book) @('books/demos/measure-and-warrant.lisp').</p>
+ through the loop, a @(see lambda) object based on the body of the @('loop$')
+ is given as the function argument of @('apply$').  Similarly, the @('UNTIL')
+ and @('WHEN') clauses of @('FOR') @('loop$')s and the @(':measure') and
+ @('FINALLY') clauses of @('DO') @('loop$')s are translated into @('lambda')
+ objects.  The functions in all those @('lambda') objects must be warranted to
+ evaluate the @('loop$') and/or prove its properties (including its guards)
+ because logically the application of an unwarranted function is
+ undefined.  (However, recall from @(see guarantees-of-the-top-level-loop) that
+ @(':program') mode functions do not need warrants, just badges, for execution
+ in the evaluation theory.)</p>
+
+ <p>The documentation for @(tsee apply$) illustrates a simple @('defun') that
+ is inadmissible because the measure theorem cannot be proved without a warrant
+ and warrants cannot be assumed during the proofs of the measure conjectures.
+ The same issue arises when one of the functions critically involved in a
+ measure conjecture is defined using a @('loop$') whose body involves a
+ user-defined function.  For a simple example of this issue and how to work
+ around it, see @(see community-book)
+ @('books/demos/measure-and-warrant.lisp').</p>
 
  <h3>Types and guards in @('loop$') expressions</h3>
 
@@ -56579,7 +57220,9 @@ forms allowed for a @('let') form are  @('ignore'), @('ignorable'), and
  (2 3 4)
  ACL2 !>(let ((max 10))
          (loop$ for x of-type integer in '(1 2 3)
-                collect :guard (and (integerp max) (< x max)) (- max x)))
+                collect
+                :guard (and (integerp max) (< x max))
+                (- max x)))
  (9 8 7)
  })
 
@@ -56656,12 +57299,28 @@ forms allowed for a @('let') form are  @('ignore'), @('ignorable'), and
   @('loop$') and the measure must be made explicit.</p>
 
   <p>Recursion is not allowed inside a @('DO') @('loop$') expression.  In fact,
-  ACL2 disallows the use of @(':loop-recursion') in the @('xargs') of any
+  ACL2 disallows the use of @(':loop$-recursion') in the @('xargs') of any
   definition whose body contains a @('DO') @('loop$').  So this topic is only
   about @('FOR') @('loop$')s.</p>
 
   <p>Some examples of @('loop$')-recursive definitions may be found in the book
   @('projects/apply/loop-recursion-examples.lisp').</p>
+
+  <p><b>Warning:</b> We advise you to use @(tsee defun$) rather than @(tsee
+  defun) when introducing a @(':logic') mode @('loop$')-recursive function.
+  When a @('loop$')-recursive function is introduced it is assigned a badge.
+  This is required because we cannot translate the body of a
+  @('loop$')-recursive function without a badge.  However, no warrant is
+  assigned by @('defun').  But it is impossible to reason about
+  applications (with @(tsee apply$)) of unwarranted functions.  Indeed, it is
+  even impossible to execute such applications in the top-level ACL2
+  read-eval-print loop.  See @(see guarantees-of-the-top-level-loop).  So a
+  @(':logic') mode @('loop$')-recursive function &mdash; which is guaranteed to
+  involve applications of itself with @('apply$') &mdash; can't be reasoned
+  about or executed (except on data not exercising the recursive calls inside
+  @('loop$')s).  These inconveniences can be avoided by using @('defun$') when
+  introducing @(':logic') mode @('loop$')-recursive functions because
+  @('defun$') expands to a @('defun') followed by a @(tsee defwarrant).</p>
 
   <p><b>Warning:</b> Even though the functions defined above are recursive,
   ACL2 does not generate induction schemes for them!  If you want to do
@@ -92623,6 +93282,11 @@ it."
  x86-64 platforms, instead of @('2000').  Thanks to Stephen Westfold for
  pointing out this oversight.</p>
 
+ <p>A new documentation topic, @(see guarantees-of-the-top-level-loop),
+ explains the logical meaning of evaluation in the ACL2 read-eval-print loop,
+ including discussion of attachments (see @(see defattach)), @(see badge)s,
+ @(see warrant)s.</p>
+
  <h3>EMACS Support</h3>
 
  <p>It is now possible to have more than one @(see acl2-doc) buffer.
@@ -97256,8 +97920,9 @@ arithmetic) for libraries of @(see books) for arithmetic reasoning.</p>")
           extension of the current world, e.g., the body calls an undefined
           function (but perhaps it can be defined), the body contains a
           @(':program') mode function (but perhaps that could be upgraded to
-          @(':logic') mode), the body contains an unbadged function symbol (but
-          perhaps @('defwarrant') could issue a warrant), etc.</li>
+          @(':logic') mode), the body contains an unbadged or unwarranted
+          function symbol (but perhaps @('defbadge') or @('defwarrant') could
+          resolve the issue), etc.</li>
 
       <li>@('(GUARD-USES-NON-COMPLIANT-FNS . fns)') - @('fns') is a list of
           function symbols used in the guard of the @('LAMBDA') object that
@@ -119429,7 +120094,9 @@ arithmetic) for libraries of @(see books) for arithmetic reasoning.</p>")
   function symbol on the correct number of suitably tame expressions with
   respect to the ilks of the function symbol, or the call of a tame @('LAMBDA')
   expression on the correct number of tame expressions.  Formally, an object
-  @('x') is a tame expression iff @('(tamep x)').</p></li>
+  @('x') is a tame expression iff @('(tamep x)').  Note that tameness implies
+  every function symbol in the expression is badged but <i>not necessarily
+  warranted</i>.</p></li>
 
   <li><p><b>suitably tame with (respect to arity and ilks)</b> aka
   @('suitably-tamep-listp'): A list of objects @('x') is <i>suitably tame</i>
@@ -119438,19 +120105,22 @@ arithmetic) for libraries of @(see books) for arithmetic reasoning.</p>")
   is a <i>quoted</i> tame function, when an ilk is @(':EXPR') the object is a
   <i>quoted</i> tame expression, and when an ilk is @('NIL') the object is a
   tame expression.  Formally, an object @('x') is suitably tame with respect to
-  @('n') and @('ilks') iff @('(suitably-tamep-listp n ilks x)').</p></li>
+  @('n') and @('ilks') iff @('(suitably-tamep-listp n ilks x)').   Note in
+  particular our use of the word ``quoted'' above.  We illustrate this in the
+  example below.</p></li>
 
   </ul>
 
-  <p>Note in particular our use of the word ``quoted'' above when defining the
-  concept of a suitably tame list of expressions.  We illustrate this in a few
-  examples below.</p>
+  <p>Note that the various notions of tameness make no mention of whether the
+  function symbols involved are in @(':program') or @(':logic') mode.  The
+  function symbols must have badges but need not have warrants.</p>
 
   <p>Intuitively, a tame expression can be built out of functions that are not
   themselves tame, e.g., scions, by making sure that every @(':FN') slot is
   occupied by a quoted tame function.  Put another way, if we were to trace the
   calls of @('apply$') while evaluating a tame expression every branch
-  eventually bottoms out on a call of a primitive.</p>
+  eventually bottoms out on a call of a primitive.  This is illustrated
+  below.</p>
 
   <h3>Examples</h3>
 
@@ -119469,6 +120139,11 @@ arithmetic) for libraries of @(see books) for arithmetic reasoning.</p>")
                       (foldr (cdr lst) fn init)))))
   })
 
+  <p>@('Sq') and @('foldr') above are defined as @(':logic') mode functions and
+  are badged and warranted (note the use of @('defun$')).  But for our purposes
+  they could have been introduced by @('defun') in @(':program') mode and then
+  badged with two calls of @('defbadge').</p>
+
   <p>As a result, we see the following badges:</p>
 
   <code>
@@ -119479,18 +120154,54 @@ arithmetic) for libraries of @(see books) for arithmetic reasoning.</p>")
   FOLDR   (APPLY$-BADGE 1 1 NIL :FN NIL)
   </code>
 
-  <p>We are going to investigate ``why'' the following expression is tame.</p>
+  <p>Consider the following expression.</p>
 
   @({
   (foldr lst (lambda$ (x y) (foldr y 'cons (list (sq x)))) nil)
   })
 
-  <p>This expression uses @('foldr') to square and reverse the order of the
-  elements of @('lst').  E.g., if @('lst') is @('(1 2 3 4)') the result is
-  @('(16 9 4 1)').</p>
+  <p>Forgetting about tameness for a moment, what does this term compute?
+  Study the definition of @('foldr') if you're not familiar with it and work it
+  out!  Answer: It collects, in reverse order, the squares of the elements of
+  @('lst').  E.g., if @('lst') is @('(1 2 3 4)') the value of the @('foldr')
+  expression above is @('(16 9 4 1)').</p>
 
-  <p>The tameness functions do not expand macros and so one should endeavor to
-  present them with fully translated terms.  So we will actually look at:</p>
+  <p>But we are interested in whether it is tame.  Tameness is a concept
+  applied to objects representing formal (fully translated) terms (or
+  components of terms in the case of ``tame functions,'' ``tame lambdas,''
+  etc.).  Saying ``<i>x</i> is a tame expression'' is just a colloquial way of
+  saying ``@('(tamep ')<i>x</i>@(')') = @('t').  So we can evaluate this
+  term in the top-level ACL2 loop,</p>
+
+  @({
+  (tamep '(foldr lst (lambda$ (x y) (foldr y 'cons (list (sq x)))) nil))
+  })
+
+  <p>and the result is @('nil') because @('lambda$') is not a ``badged function
+  symbol.'' In fact, @('lambda$') is not a function symbol.  It is a macro.
+  We're really interested in the formal translation of the @('foldr')
+  expression.  One way to understand the situation is that @('tamep') does not
+  expand macros.</p>
+
+  <p>The translation of the above term is</p>
+
+  @({
+  (FOLDR LST
+         '(LAMBDA (X Y)
+                  (DECLARE (IGNORABLE X Y))
+                  (RETURN-LAST 'PROGN
+                               '(LAMBDA$ (X Y)
+                                         (FOLDR Y 'CONS (LIST (SQ X))))
+                               (FOLDR Y 'CONS (CONS (SQ X) 'NIL))))
+         'NIL)
+  })
+
+  <p>The @('RETURN-LAST') subterm is a marker that records the original
+  user-supplied @('lambda$') expression, which is needed during compilation and
+  execution in raw Lisp.  But the value of that @('RETURN-LAST') is the
+  expected @('FOLDR') expression in its last argument.  To simplify our
+  discussion of tameness let's determine whether the following equivalent term
+  is tame.</p>
 
   @({
   (FOLDR LST
@@ -119501,18 +120212,28 @@ arithmetic) for libraries of @(see books) for arithmetic reasoning.</p>")
          'NIL)
   })
 
-  <p><i>Note: The quoted @('LAMBDA') object above is not exactly the
-  translation of the corresponding @('lambda$') expression!</i> When
-  @('lambda$') expressions are translated they are marked in a certain way for
-  benefit of execution without changing their semantics, which is accurately
-  reflected in the quoted @('LAMBDA') above.  See @(tsee lambda$).</p>
+  <p>The answer is yes, it is a tame expression.  In particular</p>
 
-  <p>The @('FOLDR') term above illustrates that even though @('FOLDR') is
-  <i>not a tame function</i> it can be used in the construction of a tame
-  expression provided, mainly, that its second argument is a quoted tame
-  function.  Indeed, the example illustrates that we can even call @('FOLDR')
-  within the @('LAMBDA') expression passed to another @('FOLDR') and still have
-  a tame expression.</p>
+  @({
+  (tamep '(FOLDR LST
+                 '(LAMBDA (X Y)
+                    (FOLDR Y
+                           'CONS
+                           (CONS (SQ X) 'NIL)))
+                 'NIL))
+  = T
+  })
+
+  <p>By the way, @('tamep') answers the same way on the quotation of the
+  actual translation of the @('foldr') term.</p>
+
+  <p>We explain below how @('tamep') computes this result.  But before we dive
+  into details consider what this example illustrates.  @('FOLDR') is <i>not a
+  tame function</i> according to the definitions above. But it can be used in
+  the construction of tame expressions provided, mainly, that its second
+  argument is a quoted tame function.  Indeed, the example illustrates that we
+  can even call @('FOLDR') within the @('LAMBDA') expression passed to another
+  @('FOLDR') and still have a tame expression.</p>
 
   <p>If we were to @(tsee trace$) the functions @('tamep'),
   @('tamep-functionp'), and @('suitably-tamep-listp'), and then call @('tamep')
@@ -119521,18 +120242,18 @@ arithmetic) for libraries of @(see books) for arithmetic reasoning.</p>")
   return @('T').  We discuss each of these calls below.</p>
 
   <code>
-  (TAMEP '(CONS (SQ X) 'NIL))                                    ; [1]
+  (tamep '(CONS (SQ X) 'NIL))                                    ; [1]
 
-  (SUITABLY-TAMEP-LISTP 3                                        ; [2]
+  (suitably-tamep-listp 3                                        ; [2]
                         '(NIL :FN NIL)
                         '(Y 'CONS (CONS (SQ X) 'NIL)))
 
-  (TAMEP '(FOLDR Y 'CONS (CONS (SQ X) 'NIL)))                    ; [3]
+  (tamep '(FOLDR Y 'CONS (CONS (SQ X) 'NIL)))                    ; [3]
 
-  (TAMEP-FUNCTIONP '(LAMBDA (X Y)                                ; [4]
+  (tamep-functionp '(LAMBDA (X Y)                                ; [4]
                             (FOLDR Y 'CONS (CONS (SQ X) 'NIL))))
 
-  (TAMEP '(FOLDR LST                                             ; [5]
+  (tamep '(FOLDR LST                                             ; [5]
                  '(LAMBDA (X Y)
                           (FOLDR Y 'CONS (CONS (SQ X) 'NIL)))
                  'NIL))
@@ -119579,7 +120300,8 @@ arithmetic) for libraries of @(see books) for arithmetic reasoning.</p>")
   the object.  But because these functions are defined in terms of @(tsee
   badge) these notions of tameness are evaluable only in the evaluation
   theory (where @(tsee warrant)s are implicitly assumed).  If you want to prove
-  that an object is tame, you may need warrant hypotheses.</p>")
+  that an object is tame, you may need warrant hypotheses.  See @(see
+  guarantees-of-the-top-level-loop).</p>")
 
 (defxdoc tau-data
   :parents (tau-system)
@@ -131568,34 +132290,45 @@ introduction-to-the-tau-system) for more information about Tau.</dd>
 
   <p>The discussion below mentions the concept of @(tsee badge)s, which are
   easily confused with warrants.  See the discussion of <b>Badges versus
-  Warrants</b> at the top of @('defwarrant').  But roughly put, badges extend
+  Warrants</b> at the top of @(tsee defbadge).  But roughly put, badges extend
   the ACL2 syntax and warrants extend the proof theory.  You'll need a badge
   for @('fn') to allow the system to syntactically analyze @('(apply$ 'fn
   ...)').  You'll need a both a badge and a warrant for @('fn') if you wish to
-  reason about that term with ACL2.</p>
+  reason about that term with ACL2.  Badges and warrants also have impact on
+  evaluation of forms in the top-level loop.  See @(see
+  guarantees-of-the-top-level-loop).</p>
 
   <p>In the ACL2 proof theory, the functions @(tsee badge) and @(tsee apply$)
-  are undefined on user-defined function symbols.  The meanings of those
-  functions can be specified by warrants.  If there is a warrant for @('fn')
-  among the hypotheses of a theorem, @('(badge 'fn)') and @('(apply$ 'fn ...)')
-  can be simplified appropriately.  We think of the warrant for @('fn') giving
-  @('badge') and @('apply$') authority to expand on @(''fn').  For reasons of
-  logical consistency not every @('fn') can have a warrant.  Warrants are
-  issued, when possible, by @(tsee defwarrant).</p>
+  are undefined on user-defined function symbols.  To be precise, when
+  presented with a user-defined function symbol, @('badge') calls the weakly
+  constrained function @('badge-userfn') and @('apply$') calls the weakly
+  constrained function @('apply$-userfn').  Warrants are terms that, if
+  available as hypotheses in a conjecture, further constrain those functions
+  for specific function symbols.  If there is a warrant for @('fn') among the
+  hypotheses of a conjecture, @('(badge 'fn)') and @('(apply$ 'fn ...)')  can
+  be simplified appropriately.  In particular, @('(badge 'fn)') is simplified
+  to the actual badge of @('fn') and @('(apply$ 'fn ...)') is simplified to the
+  appropriate application of @('fn') provided the arguments are suitably @(see
+  tame).  We think of the warrant for @('fn') giving @('badge') and @('apply$')
+  authority to expand on @(''fn').  For reasons of logical consistency not
+  every @('fn') can have a warrant.  Warrants are issued, when possible, by
+  @(tsee defwarrant).</p>
 
   <p>In the ACL2 evaluation theory &mdash; a consistent extension of the proof
   theory &mdash; all warrants issued by @('defwarrant') are implicitly assumed,
   meaning @('badge') and @('apply$') can be executed on warranted user-defined
   function symbols at the top-level of the ACL2 loop without explicit mention
-  of the warrants.  (In fact, just as the evaluation theory can -- inexplicably
-  -- execute @(':program') mode functions despite the absence of any axioms
-  about them, the evaluation theory can execute a well-formed @('apply$') on
-  any function having a @(tsee badge) even if no warrant has been issued for
-  the function.  See @(tsee defbadge).)  For a discussion of the restrictions
-  on when a @('fn') can be warranted, see @(tsee defwarrant).  This topic
-  discusses warrants <i>per se</i>, their names, their logical meaning, when
-  they must be explicitly added as hypotheses to theorems, and their
-  consistency.</p>
+  of the warrants.  In fact, just as the evaluation theory can &mdash;
+  ``magically'' &mdash; execute @(':program') mode functions despite the
+  absence of any axioms about them, the evaluation theory can execute a
+  well-formed @('apply$') on any @(':program') mode function that has a @(tsee
+  badge).  However, for a @(':logic') mode function @('fn'), the top-level loop
+  cannot evaluate @('(apply$ 'fn ...)')  unless @('(defwarrant fn)') has
+  previously succeeded.  See @(see guarantees-of-the-top-level-loop).)  For a
+  discussion of the restrictions on when a @('fn') can be warranted, see @(tsee
+  defwarrant).  This topic discusses warrants <i>per se</i>, their names, their
+  logical meaning, when they must be explicitly added as hypotheses to
+  conjectures, and their consistency.</p>
 
   <h3>Logical Definition of the Warrant of a Function</h3>
 
@@ -131638,11 +132371,6 @@ introduction-to-the-tau-system) for more information about Tau.</dd>
                                   (caddr args))))))
     :constrain t)
   })
-
-  <p>Notice that the warrant is phrased in terms of the undefined functions
-  @('badge-userfn') and @('apply$-userfn').  @('Defwarrant') will ``lift''
-  this warrant to @('badge') and @('apply$') by proving rewrite rules discussed
-  below.</p>
 
   <p>Notice also that the tameness hypothesis involves the universally
   quantified variable @('args'), but that the first conjunct of the conclusion
@@ -131720,9 +132448,9 @@ introduction-to-the-tau-system) for more information about Tau.</dd>
   })
 
   <p>Observe that these rules say that if @('(apply$-warrant-foldr)') is
-  available, then @('(badge 'FOLDR)') is @('(APPLY$-BADGE 3 1 NIL :FN NIL)')
-  and @('(apply$ 'FOLDR args)') has the naively expected behavior of calling
-  @('foldr'), provided the second element of @('args') is a
+  available as a hypothesis, then @('(badge 'FOLDR)') is @('(APPLY$-BADGE 3 1
+  NIL :FN NIL)') and @('(apply$ 'FOLDR args)') has the naively expected
+  behavior of calling @('foldr'), provided the second element of @('args') is a
   @('tamep-functionp').  Also note that the warrant hypothesis is @(tsee
   force)d in both rules.</p>
 
@@ -131732,6 +132460,9 @@ introduction-to-the-tau-system) for more information about Tau.</dd>
   @('apply$') terms are simplified whether the warrant is present or not, but
   if the warrant is not among the hypotheses and the proof is otherwise
   successful, the warrant for @('foldr') will show up in a checkpoint.</p>
+
+  <p>If no warrant has been issued for @('foldr') these terms will not
+  simplify.</p>
 
   <h3>Determining the Necessary Warrants</h3>
 
@@ -131766,7 +132497,12 @@ introduction-to-the-tau-system) for more information about Tau.</dd>
   (include-book \"projects/apply/top\" :dir :system)
 
   (defun$ sq (x) (* x x))
+  })
 
+  <p>and recall that @('collect$') is @(tsee loop$) scion logically defined
+  as</p>
+
+  @({
   (defun$ collect$ (fn lst)
     (if (endp lst)
         nil
@@ -131989,7 +132725,7 @@ introduction-to-the-tau-system) for more information about Tau.</dd>
   requirements) without explicit mention of warrants.  The crux of the proof is
   admitting a big mutually recursive clique containing versions of @('apply$')
   and all of its @(see scion)s, by inventing a measure that provably decreases
-  as @('apply$') and the scions call eachother.  The keys to that measure's
+  as @('apply$') and the scions call each other.  The keys to that measure's
   existence are the restrictions imposed by @(tsee defwarrant) and @(see
   tame)ness.  See the paper for a sketch of the proof and see the comment
   titled <tt>Essay on Admitting a Model for Apply$ and the Functions that Use
